renamed the Class WellFormed to GoodTerm, as discussed last Wed.
WellFormed has connotations of decidability. The GoodTerm predicate on
L1g will not be decidable.

Class GoodTerm (Term: Type) := goodTerm : Term  -> Prop.

This class says that the type Term comes with a predicate `goodTerm`,
which characterizes the set of terms of that language that are
guaranteed to be correctly compiled to the next stage.

This is used in the following class which declares an end to end
correctness property that we want to prove:

Class CerticoqTranslationCorrect2
  `{CerticoqLanguage2 Src SrcValue}
  `{CerticoqLanguage2 Dst DstValue}
  `{CerticoqTranslation Src Dst} :=
{
  certiGoodPres2 : goodPreserving Src Dst;
  obsePres : obsPreserving Src Dst;
}.

where  obsPreserving  is defined as

Definition obsPreserving
  `{CerticoqTranslation Src Dst}
   `{BigStepHetero Src SrcValue} `{BigStepHetero Dst DstValue}
`{GoodTerm Src}
   `{ObserveHead SrcValue} `{ObserveSubterms SrcValue}
   `{ObserveHead DstValue} `{ObserveSubterms DstValue}
  :=
   ∀ (s:Src) (sv: SrcValue),
    goodTerm s (* Randy, please note this hypothesis *)
    -> (s ⇓ sv)
    -> ∃ (dv: DstValue), (translate Src Dst s) ⇓ (Ret dv) ∧  sv ⊑ dv.

For more details on these classes, please look at
theories/common/certiClasses.v

I suggest that every language should soon declare their instance of
GoodTerm. We should start from the later phases, because the goodness of
L_i should be strong enough to imply that the translation from L_i to
L_{i+1} preserves goodness.
The instance of L1g should be strong enough to
imply goodness preservation throughout the compilation chain.

certicoq/theories/common/certiClasses.v
@@ -3,7 +3,7 @@ Require Import Common.exceptionMonad.
 Require Import Common.AstCommon.
 
 
-Class WellFormed (Term: Type) := wf : Term  -> Prop.
+Class GoodTerm (Term: Type) := goodTerm : Term  -> Prop.
 
 Generalizable Variables Src Dst Inter Term Value SrcValue DstValue InterValue.
 
@@ -46,11 +46,11 @@ Instance liftTotal `{CerticoqTotalTranslation Src Dst} : CerticoqTranslation Src
 
 
 Definition wfPreserving `{CerticoqTranslation Src Dst}
-    `{WellFormed Src} `{WellFormed Dst} : Prop := 
+    `{GoodTerm Src} `{GoodTerm Dst} : Prop := 
   ∀ (s: Src), 
-    wf s 
+    goodTerm s 
     -> match translate Src Dst s with
-      | Ret t => wf t
+      | Ret t => goodTerm t
       | Exc _ => False
       end.
 
@@ -58,13 +58,13 @@ Arguments wfPreserving Src Dst {H} {H0} {H1}.
 
 (** A Certicoq language must have an associated bigstep operational semantics and 
   a well formedness predicate (possibly \_.True) *)
-Class CerticoqLanguage `{BigStepHetero Term Value} `{WellFormed Term} := 
+Class CerticoqLanguage `{BigStepHetero Term Value} `{GoodTerm Term} := 
 {
   (* Sensible, but not needed yet.
   wfPreserved : forall (s v : Term), 
-    wf s
+    goodTerm s
     -> s ⇓ v
-    -> wf v
+    -> goodTerm v
   *)
 }.
 
@@ -82,10 +82,10 @@ Arguments CerticoqLanguage Term {Value} {H} {H0}.
 
 Definition bigStepPreserving `{CerticoqTranslation Src Dst} 
   `{CerticoqTranslation SrcValue DstValue}
-   `{BigStepHetero Src SrcValue} `{BigStepHetero Dst DstValue} `{WellFormed Src}
+   `{BigStepHetero Src SrcValue} `{BigStepHetero Dst DstValue} `{GoodTerm Src}
   :=
    ∀ (s:Src) (sv: SrcValue), 
-    wf s 
+    goodTerm s 
     -> s ⇓ sv
     -> (translate Src Dst s) ⇓ (translate SrcValue DstValue sv).
 
@@ -110,9 +110,9 @@ Global Instance composeTranslation `{CerticoqTranslation Src Inter}
 
 
 Lemma composePreservesWf (Src Inter Dst: Type)
-  {wfi: WellFormed Inter}
-  {wfs: WellFormed Src}
-  {wft: WellFormed Dst}
+  {wfi: GoodTerm Inter}
+  {wfs: GoodTerm Src}
+  {wft: GoodTerm Dst}
   {t1 : CerticoqTranslation Src Inter}
   {t2 : CerticoqTranslation Inter Dst} :
 wfPreserving Src Inter
@@ -204,26 +204,26 @@ Notation "s ⊑ t" := (obsLe s t) (at level 65).
 (* Similar to what Zoe suggested on 	Wed, Aug 17, 2016 at 8:57 AM *)
 Definition obsPreserving 
   `{CerticoqTranslation Src Dst} 
-   `{BigStepHetero Src SrcValue} `{BigStepHetero Dst DstValue} `{WellFormed Src}
+   `{BigStepHetero Src SrcValue} `{BigStepHetero Dst DstValue} `{GoodTerm Src}
    `{ObserveHead SrcValue} `{ObserveSubterms SrcValue} 
    `{ObserveHead DstValue} `{ObserveSubterms DstValue}
   :=
    ∀ (s:Src) (sv: SrcValue), 
-    wf s 
+    goodTerm s 
     -> (s ⇓ sv)
     -> ∃ (dv: DstValue), (translate Src Dst s) ⇓ (Ret dv) ∧  sv ⊑ dv.
 
 Global Arguments obsPreserving Src Dst {H} {SrcValue} {H0} {DstValue} {H1} {H2} {H3} {H4} {H5} {H6}.
 
-Class CerticoqLanguage2 `{BigStepHetero Term Value} `{WellFormed Term} 
+Class CerticoqLanguage2 `{BigStepHetero Term Value} `{GoodTerm Term} 
    `{ObserveHead Value} `{ObserveSubterms Value} 
 := 
 {
   (* Sensible, but not needed yet.
   wfPreserved : forall (s v : Term), 
-    wf s
+    goodTerm s
     -> s ⇓ v
-    -> wf v
+    -> goodTerm v
   *)
 }.
 
@@ -371,14 +371,14 @@ Qed.
 
 Lemma obsPreservingWeakenObs
   `{CerticoqTranslation Src Dst} 
-   `{BigStepHetero Src SrcValue} `{BigStepHetero Dst DstValue} `{WellFormed Src}
+   `{BigStepHetero Src SrcValue} `{BigStepHetero Dst DstValue} `{GoodTerm Src}
    `{os: ObserveHead Obs1 SrcValue} `{ObserveSubterms SrcValue} 
    `{od: ObserveHead Obs1 DstValue} `{ObserveSubterms DstValue}:
     obsPreserving Obs1 Src Dst
     -> obsPreserving Obs2 Src Dst.
 Proof.
-  intros Ho ? ? Hwf He.
-  specialize (Ho _ _ Hwf He). clear Hwf He.
+  intros Ho ? ? HgoodTerm He.
+  specialize (Ho _ _ HgoodTerm He). clear HgoodTerm He.
   destruct Ho as [dv Hev].
   exists dv.
   split;[tauto|]. apply proj2 in Hev.
@@ -400,7 +400,7 @@ Local Instance certicoqTranslationCorrectWeakenObs
       (CerticoqLanguage2WeakenObs Ld).
 Proof using.
   destruct Ht1.
-  constructor;[assumption|]. (* wf is independent of observations *)
+  constructor;[assumption|]. (* goodTerm is independent of observations *)
   apply obsPreservingWeakenObs. assumption.
 Qed.
 
@@ -512,7 +512,7 @@ Lemma bigStepPreservingReflecting
   {_:bigStepPreserving Src Dst} :
   (deterministicBigStep Dst)
   -> ∀ (s:Src), 
-    wf s
+    goodTerm s
     -> normalizes s
     -> bigStepReflecting Src Dst s.
 Proof.
